Remove the unused `low` and `high` arguments to the driver program. Now the driver searches the whole array. The IR correctness theorem will compare the IR implementation to the Lean implentation when run on the entire array

BinarySearch/ProgramDriver.lean
@@ -10,9 +10,9 @@ open  BinarySearch.Interp BinarySearch.Program
 
 private def C : Nat := 10
 
-def binarySearch (arr : Array Nat) (target : Nat) (low high : Nat) : Result :=
+def binarySearch (arr : Array Nat) (target : Nat) : Result :=
   let env := Environment.mk arr target
-  let state := State.mk low high 0
-  interp env state (C*(high - low) + C) binarySearchIR
+  let state := State.mk 0 0 0
+  interp env state (C*arr.size + C) binarySearchIR
 
 end BinarySearch.ProgramDriver
