BinarySearch/ProgramTest.lean
@@ -9,11 +9,11 @@ open BinarySearch.ProgramDriver open BinarySearch.Interp
 
 def testArray : Array Nat := #[1, 3, 5, 7, 7, 9]
 
-#guard binarySearch testArray 5 0 testArray.size == Result.return_index 2
-#guard binarySearch testArray 2 0 testArray.size == Result.return_none
-#guard binarySearch testArray 9 0 testArray.size == Result.return_index 5
-#guard binarySearch testArray 1 0 testArray.size == Result.return_index 0
-#guard binarySearch testArray 0 0 testArray.size == Result.return_none
-#guard binarySearch testArray 7 0 testArray.size == Result.return_index 3
+#guard binarySearch testArray 5 == Result.return_index 2
+#guard binarySearch testArray 2 == Result.return_none
+#guard binarySearch testArray 9 == Result.return_index 5
+#guard binarySearch testArray 1 == Result.return_index 0
+#guard binarySearch testArray 0 == Result.return_none
+#guard binarySearch testArray 7 == Result.return_index 3
 
 end BinarySearch.ProgramTest
